theories/case_studies/multiuser_kvs/kvs_spec_addOrUpdate_safe.v
@@ -17,7 +17,7 @@ Section KVS_spec_addOrUpdate_safe.
     {cstackg : CSTACKG Σ}
     `{MP: MachineParameters}
     {swlayout : switcherLayout}
-    {KVS_layout : kvsLayout} {KVS_users: kvs_users} {KVS_namespaces : kvs_namespaces}
+    {KVS_layout : kvsLayout} {KVS_layout_WF : kvsLayoutWf} {KVS_users: kvs_users} {KVS_namespaces : kvs_namespaces}
   .
 
   (*** Specification from unknown *)
